execution/examples/EscrowSolana.v
@@ -1,0 +1,904 @@
+(* This file defines a simple escrow contract based on the "safe remote
+purchase" example in Solidity's docs. This contract allows a seller to sell an
+item in a trustless setting assuming economically rational actors. With the
+premise that the seller wants to sell an item for 1 ETH, the contract works in
+the following way:
+
+1. The seller deploys the contract and commits 2 ETH.
+2. The buyer commits 2 ETH before the deadline.
+3. The seller hands over the item (outside of the smart contract).
+4. The buyer confirms he has received the item. He gets 1 ETH back
+while the seller gets 3 ETH back.
+
+If the buyer does not commit the funds, the seller gets his money back after the
+deadline. The economic rationality shows up in our assumption that the seller
+will confirm he has received the item to get his own funds back. *)
+
+From Coq Require Import List.
+From Coq Require Import Bool.
+From Coq Require Import ZArith.
+From Coq Require Import Permutation.
+From Coq Require Import Psatz.
+From ConCert.Execution Require Import BlockchainSolanav2.
+From ConCert.Execution Require Import Extras.
+From ConCert.Execution Require Import Monads.
+From ConCert.Execution Require Import ResultMonad.
+From ConCert.Execution Require Import Serializable.
+From ConCert.Utils Require Import Automation.
+From ConCert.Utils Require Import RecordUpdate.
+
+Import ListNotations.
+Import RecordSetNotations.
+
+Section EscrowSolana.
+Context `{Base : ChainBase}.
+
+Set Nonrecursive Elimination Schemes.
+
+Record Setup :=
+  build_setup {
+      setup_buyer : Address;
+    }.
+
+Inductive NextStep :=
+(* Waiting for buyer to commit itemvalue * 2 *)
+| buyer_commit
+(* Waiting for buyer to confirm item received *)
+| buyer_confirm
+(* Waiting for buyer and seller to withdraw their funds. *)
+| withdrawals
+(* No next step, sale is done. *)
+| no_next_step.
+
+Record State :=
+  build_state {
+      last_action : nat;
+      next_step : NextStep;
+      seller : Address;
+      buyer : Address;
+      seller_withdrawable : Amount;
+      buyer_withdrawable : Amount;
+      is_initialized : bool;
+    }.
+
+Inductive MsgType :=
+| init_escrow
+| commit_money
+| confirm_item_received
+| withdraw.
+
+Record Msg :=
+  build_message {
+    instruction : option MsgType;
+    setup : option SerializedValue;
+    amount : option SerializedValue;
+  }.
+
+Inductive EscrowError : Type :=
+| InvalidInstruction
+| NotRentExempt
+| InvalidAmount
+| InvalidAccounts
+| ProgramError. (* TODO: Should be Program error from BlockchainSolana *) 
+
+MetaCoq Run (make_setters State).
+MetaCoq Run (make_setters Msg).
+
+Global Instance Setup_serializable : Serializable Setup :=
+  Derive Serializable Setup_rect<build_setup>.
+
+Global Instance NextStep_serializable : Serializable NextStep :=
+  Derive Serializable NextStep_rect<buyer_commit, buyer_confirm, withdrawals, no_next_step>.
+
+Global Instance State_serializable : Serializable State :=
+  Derive Serializable State_rect<build_state>.
+
+Global Instance MsgType_serializable : Serializable MsgType :=
+  Derive Serializable MsgType_rect<init_escrow, commit_money, confirm_item_received, withdraw>.
+
+Global Instance Msg_serializable : Serializable Msg :=
+  Derive Serializable Msg_rect<build_message>.
+
+Open Scope Z.
+
+Definition escrow_init (chain : Chain) (accounts : list AccountInfo) (setup : Setup)
+  : result (list ActionBody) EscrowError :=
+  let buyer_address := setup_buyer setup in
+
+  let seller_account_opt := (nth_error accounts 0) in
+  let temp_token_account_opt := (nth_error accounts 1) in
+  let token_to_receive_account_opt := (nth_error accounts 2) in
+  let escrow_account_opt := (nth_error accounts 3) in
+  let rent_sysvar_account_opt := (nth_error accounts 4) in
+  let token_program_account_opt := (nth_error accounts 5) in
+
+  match seller_account_opt with
+  | Some seller_account =>
+        match temp_token_account_opt with
+        | Some temp_token_account =>
+              match token_to_receive_account_opt with
+              | Some token_to_receive_account =>
+                  match escrow_account_opt with
+                  | Some escrow_account =>
+                      match rent_sysvar_account_opt with
+                      | Some rent_sysvar_account =>
+                          match token_program_account_opt with
+                          | Some token_program_account =>
+                              do if (account_is_signer seller_account) then Ok tt else Err InvalidAccounts;
+                              do if ((account_owner_address seller_account) =? (account_address token_program_account))%address then Ok tt else Err ProgramError;
+                              (* TODO: HERE SHOULD CHECK RENT EXEMPT *)
+                              let escrow_account_deserialize_state := ((@deserialize State _) (account_state escrow_account)) in  
+                              do match escrow_account_deserialize_state with 
+                                  | Some st => if (is_initialized st) then Err ProgramError else Ok tt
+                                  | None => Ok tt
+                              end;
+
+    
+                              let initialized_state := (build_state
+                                  (current_slot chain)
+                                  buyer_commit
+                                  (account_address seller_account)
+                                  buyer_address
+                                  0 0 true)
+                                in
+                                          
+                              
+(*                               do escrow_account<|account_state := (@serialize State _) initialized_state|>; *)
+
+                              let seller_account_balance := (account_balance temp_token_account) in
+                              do if (buyer_address =? (account_address seller_account))%address then Err InvalidAccounts else Ok tt;
+                              do if seller_account_balance =? 0 then Err InvalidAmount else Ok tt;
+                              do if Z.even seller_account_balance then Ok tt else Err InvalidAmount ;
+                            
+                              Ok ([act_special_call (account_address token_program_account)
+                                      (transfer_ownership (account_address token_to_receive_account) (account_address token_program_account))])
+                          | None => Err InvalidAccounts
+                          end
+                      | None => Err InvalidAccounts
+                    end
+                  | None => Err InvalidAccounts
+                  end
+              | None => Err InvalidAccounts
+              end
+        | None => Err InvalidAccounts
+        end
+  | None => Err InvalidAccounts
+  end.
+
+Definition escrow_commit_money (chain : Chain) (accounts : list AccountInfo) (amount : Amount) : result (list ActionBody) EscrowError :=
+  let buyer_account_opt := (nth_error accounts 0) in
+  let temp_token_account_opt := (nth_error accounts 1) in
+  let token_to_receive_account_opt := (nth_error accounts 2) in
+  let escrow_account_opt := (nth_error accounts 3) in
+  let rent_sysvar_account_opt := (nth_error accounts 4) in
+  let token_program_account_opt := (nth_error accounts 5) in
+
+  match buyer_account_opt with
+  | Some buyer_account =>
+        match temp_token_account_opt with
+        | Some temp_token_account =>
+              match token_to_receive_account_opt with
+              | Some token_to_receive_account =>
+                  match escrow_account_opt with
+                  | Some escrow_account =>
+                      match rent_sysvar_account_opt with
+                      | Some rent_sysvar_account =>
+                          match token_program_account_opt with
+                          | Some token_program_account =>
+                              let escrow_account_deserialize_state := ((@deserialize State _) (account_state escrow_account)) in
+                              match escrow_account_deserialize_state with 
+                                | Some st => 
+                                    do if (is_initialized st) then Ok tt else Err ProgramError;
+                                    do if (buyer st =? account_address buyer_account)%address then Ok tt else Err InvalidAccounts;
+
+                                    let expected := amount * 2 in
+                                    do if (account_balance buyer_account >=? expected) then Ok tt else Err InvalidAmount;
+
+                                    let state := st<|next_step := buyer_confirm|>
+                                                   <|last_action := current_slot chain|> in
+                                    
+                                    (* escrow_account<|account_state := (@serialize State _) initialized_state|>; *)
+
+                                    Ok ([])
+                                  | None => Err InvalidAccounts
+                                end
+                          | None => Err InvalidAccounts
+                          end
+                      | None => Err InvalidAccounts
+                    end
+                  | None => Err InvalidAccounts
+                  end
+              | None => Err InvalidAccounts
+              end
+        | None => Err InvalidAccounts
+        end
+  | None => Err InvalidAccounts
+  end.
+
+Definition escrow_confirm_item_received (chain : Chain) (accounts : list AccountInfo) (amount : Amount) : result (list ActionBody) EscrowError :=
+  let buyer_account_opt := (nth_error accounts 0) in
+  let temp_token_account_opt := (nth_error accounts 1) in
+  let token_to_receive_account_opt := (nth_error accounts 2) in
+  let escrow_account_opt := (nth_error accounts 3) in
+  let rent_sysvar_account_opt := (nth_error accounts 4) in
+  let token_program_account_opt := (nth_error accounts 5) in
+
+  match buyer_account_opt with
+  | Some buyer_account =>
+        match temp_token_account_opt with
+        | Some temp_token_account =>
+              match token_to_receive_account_opt with
+              | Some token_to_receive_account =>
+                  match escrow_account_opt with
+                  | Some escrow_account =>
+                      match rent_sysvar_account_opt with
+                      | Some rent_sysvar_account =>
+                          match token_program_account_opt with
+                          | Some token_program_account =>
+                              let escrow_account_deserialize_state := ((@deserialize State _) (account_state escrow_account)) in
+                              match escrow_account_deserialize_state with 
+                                | Some st => 
+                                    do if (is_initialized st) then Ok tt else Err ProgramError;
+                                    do if (buyer st =? account_address buyer_account)%address then Ok tt else Err InvalidAccounts;
+
+                                    let state := st<|next_step := withdrawals|>
+                                                   <|buyer_withdrawable := amount|>
+                                                   <|seller_withdrawable := amount * 3|> in
+                                    
+                                    (* escrow_account<|account_state := (@serialize State _) initialized_state|>; *)
+
+                                    Ok ([])
+                                  | None => Err InvalidAccounts
+                                end
+                          | None => Err InvalidAccounts
+                          end
+                      | None => Err InvalidAccounts
+                    end
+                  | None => Err InvalidAccounts
+                  end
+              | None => Err InvalidAccounts
+              end
+        | None => Err InvalidAccounts
+        end
+  | None => Err InvalidAccounts
+  end.
+
+Definition escrow_withdraw (chain : Chain) (accounts : list AccountInfo) (amount : Amount) : result (list ActionBody) EscrowError :=
+  let participant_account_opt := (nth_error accounts 0) in
+  let temp_token_account_opt := (nth_error accounts 1) in
+  let token_to_receive_account_opt := (nth_error accounts 2) in
+  let escrow_account_opt := (nth_error accounts 3) in
+  let rent_sysvar_account_opt := (nth_error accounts 4) in
+  let token_program_account_opt := (nth_error accounts 5) in
+
+  match participant_account_opt with
+  | Some participant_account =>
+        match temp_token_account_opt with
+        | Some temp_token_account =>
+              match token_to_receive_account_opt with
+              | Some token_to_receive_account =>
+                  match escrow_account_opt with
+                  | Some escrow_account =>
+                      match rent_sysvar_account_opt with
+                      | Some rent_sysvar_account =>
+                          match token_program_account_opt with
+                          | Some token_program_account =>
+                              let escrow_account_deserialize_state := ((@deserialize State _) (account_state escrow_account)) in
+                              match escrow_account_deserialize_state with 
+                                | Some st => 
+                                    do if (is_initialized st) then Ok tt else Err ProgramError;
+
+                                    match next_step st with 
+                                    | buyer_commit =>
+                                      do if (last_action st + 50 <? current_slot chain)%nat then Err ProgramError else Ok tt;
+                                      do if ((account_address participant_account) =? seller st)%address then Ok tt else Err InvalidAccounts;
+                                      let balance := account_balance escrow_account in
+                                      (* state<|next_step := no_next_step|> *)
+                                      Ok ([act_transfer (seller st) balance])
+                                    | _ =>
+
+                                      do '(to_pay, new_state) <-
+                                         match (account_address participant_account) =? (buyer st), 
+                                               (account_address participant_account) =? (seller st) with
+                                         | true, _ => Ok (buyer_withdrawable st, st<|buyer_withdrawable := 0|>)
+                                         | _, true => Ok (seller_withdrawable st, st<|seller_withdrawable := 0|>)
+                                         | _, _ => Err ProgramError
+                                         end%address;
+                                      
+                                    
+                                      do if to_pay >? 0 then Ok tt else Err ProgramError;
+                                      let new_state :=
+                                          if (buyer_withdrawable new_state =? 0) && (seller_withdrawable new_state =? 0)
+                                          then new_state<|next_step := no_next_step|>
+                                          else new_state in
+
+                                      (* escrow_account<|account_state := (@serialize State _) new_state|>; *)
+
+                                      Ok ([act_transfer (account_address participant_account) 0])
+                                    end
+                                  | None => Err InvalidAccounts
+                                end
+                          | None => Err InvalidAccounts
+                          end
+                      | None => Err InvalidAccounts
+                    end
+                  | None => Err InvalidAccounts
+                  end
+              | None => Err InvalidAccounts
+              end
+        | None => Err InvalidAccounts
+        end
+  | None => Err InvalidAccounts
+  end.
+
+Definition process (chain : Chain) (accounts : list AccountInfo) (msg : option Msg) : result (list ActionBody) EscrowError :=
+    (* TODO: Setup should come inside of the MSG *)
+    match msg with
+    | Some message =>
+        match instruction message with
+        | Some init_escrow =>
+            match setup message with
+            | Some ser_setup => 
+                match ((@deserialize Setup _) ser_setup) with 
+                | Some setup =>
+                    escrow_init chain accounts setup
+                | None => Err ProgramError
+                end
+            | None => Err ProgramError
+            end 
+        | Some commit_money => 
+            match amount message with
+            | Some ser_amount => 
+              match ((@deserialize Amount _) ser_amount) with 
+              | Some amount =>
+                  escrow_commit_money chain accounts amount
+              | None => Err ProgramError
+              end
+            | None => Err ProgramError
+            end 
+        | Some confirm_item_received =>
+            match amount message with
+            | Some ser_amount => 
+              match ((@deserialize Amount _) ser_amount) with 
+              | Some amount =>
+                escrow_confirm_item_received chain accounts amount
+              | None => Err ProgramError
+              end
+            | None => Err ProgramError
+            end 
+        | Some withdraw =>
+            match amount message with
+           | Some ser_amount => 
+             match ((@deserialize Amount _) ser_amount) with 
+              | Some amount =>
+                  escrow_withdraw chain accounts amount
+            | None => Err ProgramError
+            end
+            | None => Err ProgramError
+            end
+        | None => Err ProgramError
+        end
+    | None => Err InvalidInstruction
+    end.
+
+Definition contract : Contract Msg State :=
+  build_contract process.
+
+Section Theories.
+  Lemma no_self_calls bstate caddr :
+    reachable bstate ->
+    env_contracts bstate caddr = Some (Escrow.contract : WeakContract) ->
+    Forall (fun abody => match abody with
+                         | act_transfer to _ => (to =? caddr)%address = false
+                         | _ => False
+                         end) (outgoing_acts bstate caddr).
+  Proof.
+    contract_induction; intros; cbn in *; auto.
+    - now inversion IH.
+    - apply Forall_app; split; try tauto.
+      clear IH.
+      unfold receive in receive_some.
+      destruct_match as [[]|] in receive_some; try congruence.
+      + destruct_match in receive_some; try congruence.
+        destruct_match in receive_some; cbn in *; try congruence.
+        destruct_match in receive_some; cbn in *; try congruence.
+        inversion_clear receive_some; auto.
+      + destruct_match in receive_some; try congruence.
+        destruct_match in receive_some; cbn in *; try congruence.
+        destruct_match in receive_some; cbn in *; try congruence.
+        inversion_clear receive_some; auto.
+      + destruct_match in receive_some; try congruence.
+        * destruct_match in receive_some; cbn in *; try congruence.
+          destruct_match in receive_some; cbn in *; try congruence.
+          destruct (address_eqb_spec (ctx_from ctx) (seller prev_state)) as
+              [<-|]; cbn in *; try congruence.
+          inversion_clear receive_some.
+          constructor; try constructor.
+          apply address_eq_ne; auto.
+        * destruct_match in receive_some; cbn in *; try congruence.
+          destruct_match in receive_some; cbn in *; try congruence.
+          destruct_match in receive_some.
+          destruct_match in receive_some; cbn in *; try congruence.
+          inversion_clear receive_some.
+          constructor; try constructor.
+          apply address_eq_ne; auto.
+    - inversion_clear IH as [|? ? head_not_me tail_not_me].
+      apply Forall_app; split; auto; clear tail_not_me.
+      destruct head; try contradiction.
+      destruct action_facts as [? [? ?]].
+      destruct_address_eq; congruence.
+    - now rewrite <- perm.
+    - instantiate (DeployFacts := fun _ _ => True).
+      instantiate (CallFacts := fun _ _ _ _ => True).
+      instantiate (AddBlockFacts := fun _ _ _ _ _ _ => True).
+      unset_all; subst; cbn in *.
+      destruct_chain_step; auto.
+      destruct_action_eval; auto.
+  Qed.
+
+  Definition txs_to (to : Address) (txs : list Tx) : list Tx :=
+    filter (fun tx => (tx_to tx =? to)%address) txs.
+
+  Arguments txs_to : simpl never.
+
+  Lemma txs_to_cons addr tx txs :
+    txs_to addr (tx :: txs) =
+    if (tx_to tx =? addr)%address then
+      tx :: txs_to addr txs
+    else
+      txs_to addr txs.
+  Proof. reflexivity. Qed.
+
+  Definition txs_from (from : Address) (txs : list Tx) : list Tx :=
+    filter (fun tx => (tx_from tx =? from)%address) txs.
+
+  Arguments txs_from : simpl never.
+
+  Lemma txs_from_cons addr tx txs :
+    txs_from addr (tx :: txs) =
+    if (tx_from tx =? addr)%address then
+      tx :: txs_from addr txs
+    else
+      txs_from addr txs.
+  Proof. reflexivity. Qed.
+
+  Local Open Scope bool.
+  Definition buyer_confirmed (inc_calls : list (ContractCallInfo Msg)) buyer :=
+    existsb (fun call => (call_from call =? buyer)%address &&
+                         match call_msg call with
+                         | Some confirm_item_received => true
+                         | _ => false
+                         end) inc_calls.
+
+  Definition transfer_acts_to addr acts :=
+    filter (fun a => match a with
+                     | act_transfer to _ => (to =? addr)%address
+                     | _ => false
+                     end) acts.
+
+  Arguments transfer_acts_to : simpl never.
+
+  Lemma transfer_acts_to_cons addr act acts :
+    transfer_acts_to addr (act :: acts) =
+    if match act with
+       | act_transfer to _ => (to =? addr)%address
+       | _ => false
+       end
+    then
+      act :: transfer_acts_to addr acts
+    else
+      transfer_acts_to addr acts.
+  Proof. reflexivity. Qed.
+
+  Definition money_to
+             {bstate_from bstate_to}
+             (trace : ChainTrace bstate_from bstate_to)
+             caddr addr :=
+    sumZ tx_amount (txs_to addr (outgoing_txs trace caddr)) +
+    sumZ act_body_amount (transfer_acts_to addr (outgoing_acts bstate_to caddr)).
+
+  Lemma escrow_correct_strong bstate caddr (trace : ChainTrace empty_state bstate) :
+    env_contracts bstate caddr = Some (Escrow.contract : WeakContract) ->
+    exists (cstate : State)
+           (depinfo : DeploymentInfo Setup)
+           (inc_calls : list (ContractCallInfo Msg)),
+      deployment_info Setup trace caddr = Some depinfo /\
+      contract_state bstate caddr = Some cstate /\
+      incoming_calls Msg trace caddr = Some inc_calls /\
+      let item_worth := deployment_amount depinfo / 2 in
+      let seller_addr := deployment_from depinfo in
+      let buyer_addr := setup_buyer (deployment_setup depinfo) in
+      deployment_amount depinfo = 2 * item_worth /\
+      item_worth > 0 /\
+      seller cstate = seller_addr /\
+      buyer cstate = buyer_addr /\
+      buyer_addr <> seller_addr /\
+      forallb (fun act => match act with
+                         | act_transfer _ _ => true
+                         | _ => false
+                         end) (outgoing_acts bstate caddr) = true /\
+      match next_step cstate with
+      | buyer_commit =>
+        env_account_balances bstate caddr = 2 * item_worth /\
+        outgoing_acts bstate caddr = [] /\
+        outgoing_txs trace caddr = [] /\
+        inc_calls = []
+
+      | buyer_confirm =>
+        env_account_balances bstate caddr = 4 * item_worth /\
+        outgoing_acts bstate caddr = [] /\
+        outgoing_txs trace caddr = [] /\
+        exists origin, inc_calls = [build_call_info origin buyer_addr (2 * item_worth) (Some commit_money)]
+
+      | withdrawals =>
+        buyer_confirmed inc_calls buyer_addr = true /\
+        (exists origin, filter (fun c => negb (call_amount c =? 0)%Z ) inc_calls =
+        [build_call_info origin buyer_addr (2 * item_worth) (Some commit_money)]) /\
+        money_to trace caddr seller_addr + seller_withdrawable cstate = 3 * item_worth /\
+        money_to trace caddr buyer_addr + buyer_withdrawable cstate = 1 * item_worth
+
+      | no_next_step =>
+        buyer_confirmed inc_calls buyer_addr = true /\
+        (exists origin, filter (fun c => negb (call_amount c =? 0)%Z) inc_calls =
+        [build_call_info origin buyer_addr (2 * item_worth) (Some commit_money)]) /\
+        money_to trace caddr seller_addr = 3 * item_worth /\
+        money_to trace caddr buyer_addr = 1 * item_worth \/
+
+        (exists origin, inc_calls = [build_call_info origin seller_addr 0 (Some withdraw)]) /\
+        money_to trace caddr seller_addr = 2 * item_worth /\
+        money_to trace caddr buyer_addr = 0
+      end.
+  Proof.
+    unfold money_to.
+    contract_induction; cbn in *; intros.
+    - (* New block *)
+      auto.
+    - (* Deployment *)
+      unfold Escrow.init in *.
+      destruct (address_eqb_spec (setup_buyer setup) (ctx_from ctx));
+        cbn in *; try congruence.
+      destruct (ctx_amount ctx =? 0) eqn:amount_some; cbn in *; try congruence.
+      destruct (Z.even (ctx_amount ctx)) eqn:amount_even; cbn in *; try congruence.
+      inversion init_some; subst; clear init_some.
+      cbn.
+      assert (2 * (ctx_amount ctx / 2) > 0 -> ctx_amount ctx / 2 > 0) by lia.
+      enough (2 * (ctx_amount ctx / 2) > 0 /\
+              ctx_amount ctx = 2 * (ctx_amount ctx / 2)) by tauto.
+      assert (ctx_amount ctx mod 2 = 0).
+      {
+        rewrite Zeven_mod in amount_even.
+        unfold Zeq_bool in *.
+        destruct_match eqn:amount_mod_2 in amount_even; try congruence; auto.
+        destruct (Z.compare_spec (ctx_amount ctx mod 2) 0); auto; try congruence.
+      }
+      rewrite <- (Z_div_exact_2 (ctx_amount ctx) 2) by (auto; lia).
+      split; auto.
+      instantiate (DeployFacts := fun _ ctx => ctx_amount ctx >= 0);
+        subst DeployFacts; cbn in *.
+      apply Z.eqb_neq in amount_some.
+      lia.
+    - (* Transfer from contract to someone *)
+      repeat rewrite txs_to_cons.
+      do 5 (split; try tauto).
+      destruct IH as [_ [_ [_ [<- [_ [only_transfers IH]]]]]].
+      apply andb_prop in only_transfers.
+      split; try tauto.
+      destruct only_transfers as [is_transfer _].
+      destruct out_act; try congruence.
+      destruct tx_act_match as [<- [<- _]].
+      repeat rewrite transfer_acts_to_cons in *.
+      destruct (next_step cstate).
+      + intuition congruence.
+      + intuition congruence.
+      + (* Transfer while next_step is withdraw; so seller or buyer withdrew *)
+        do 2 (split; try tauto).
+        destruct IH as [_ [_ [? ?]]].
+        destruct_address_eq; cbn in *; lia.
+      + (* Transfer while next_step is no_next_step; action moved from queue to txs *)
+        destruct IH as [IH | IH]; [left|right].
+        * do 2 (split; try tauto).
+          destruct IH as [_ [? ?]].
+          destruct_address_eq; cbn in *; lia.
+        * split; try tauto.
+          destruct IH as [_ ?].
+          destruct_address_eq; cbn in *; lia.
+    - (* Call from someone else *)
+      do 2 (split; try tauto).
+      unfold Escrow.receive in *.
+      set (item_worth := deployment_amount dep_info / 2) in *.
+      destruct msg as [[| |]|].
+      + (* Some commit_money *)
+        destruct (next_step prev_state); try congruence.
+        destruct (address_eqb_spec (ctx_from ctx) (buyer prev_state)) as [->|];
+          cbn in *; try congruence.
+        destruct (ctx_amount ctx =? _) eqn:proper_amount in receive_some;
+          cbn in *; try congruence.
+        inversion_clear receive_some.
+        cbn.
+        do 4 (split; try tauto).
+        destruct IH as [deployed_even [_ [_ [-> [_ [_ [balance_eq [-> [-> ->]]]]]]]]].
+        apply Z.eqb_eq in proper_amount.
+        rewrite balance_eq in proper_amount.
+        rewrite proper_amount.
+        replace (ctx_contract_balance _) with (2 * item_worth + 2 * item_worth / 2 * 2) by lia.
+        rewrite <- Z.mul_comm.
+        rewrite Z.div_mul by lia.
+        repeat split;eauto.
+        lia.
+      + (* Some confirm_item_received *)
+        destruct_match in receive_some; cbn in *; try congruence.
+        destruct (address_eqb_spec (ctx_from ctx) (buyer prev_state)) as [->|];
+          cbn in *; try congruence.
+        destruct (ctx_amount ctx =? 0) eqn:zero_amount in receive_some;
+          cbn in *; try congruence.
+        inversion_clear receive_some.
+        cbn.
+        do 4 (split; try tauto).
+        destruct IH as [deployed_even [? [<- [<- [_ [_ [balance_eq [-> [-> H]]]]]]]]].
+        destruct H as [origin Hcalls].
+        rewrite Hcalls.
+        rewrite address_eq_refl.
+        cbn.
+        split; auto.
+        unfold txs_to, transfer_acts_to; cbn.
+        apply Z.eqb_eq in zero_amount.
+        rewrite zero_amount in *.
+        replace (ctx_contract_balance _) with (4 * item_worth) in * by lia.
+        rewrite (Z.mul_comm 4).
+        rewrite Z.div_mul by lia.
+        destruct (Z.eqb_spec (2 * item_worth) 0); cbn in *; try lia.
+        repeat split; eauto;lia.
+      + (* Some withdraw. Can be sent while next_step is either
+           commit_money or withdrawals. *)
+        destruct_match eqn:prev_next_step in receive_some;
+          cbn -[Nat.ltb] in *; try congruence.
+        * (* next_step was commit_money, so seller is withdrawing money
+          because buyer did not commit anything. *)
+          destruct (ctx_amount ctx =? 0) eqn:zero_amount in receive_some;
+            cbn -[Nat.ltb] in *; try congruence.
+          apply Z.eqb_eq in zero_amount.
+          rewrite zero_amount in *.
+          destruct_match in receive_some; cbn in *; try congruence.
+          destruct (address_eqb_spec (ctx_from ctx) (seller prev_state))
+            as [->|]; cbn in *; try congruence.
+          inversion_clear receive_some; cbn.
+          do 4 (split; try tauto).
+          (* In this case we go to no_next_step state without buyer having confirmed anything *)
+          right.
+          destruct IH as [_ [_ [<- [_ [? [_ [? [-> [-> ->]]]]]]]]].
+          unfold txs_to, transfer_acts_to.
+          cbn.
+          rewrite address_eq_refl, address_eq_ne by auto.
+          cbn.
+          split; eauto; lia.
+        * (* next_step was withdrawals, so either seller or buyer is withdrawing money.
+             This might put us into next_step = no_next_step. *)
+          destruct (ctx_amount ctx =? 0) eqn:zero_amount in receive_some;
+            cbn -[Nat.ltb] in *; try congruence.
+          apply Z.eqb_eq in zero_amount.
+          rewrite zero_amount in *.
+          destruct (address_eqb_spec (ctx_from ctx) (buyer prev_state))
+            as [->|]; [|destruct (address_eqb_spec (ctx_from ctx) (seller prev_state))
+                         as [->|]; cbn in *; try congruence].
+          -- (* Buyer withdrawing *)
+            cbn in *.
+            destruct_match in receive_some; cbn in *; try congruence.
+            inversion_clear receive_some; cbn.
+            apply and_assoc; split; [destruct_match; tauto|].
+            do 2 (split; try tauto).
+            destruct (Z.eqb_spec (seller_withdrawable prev_state) 0) as [seller_done|].
+            ++ (* No one has more to withdrew, next_step is no_next_step now, so establish
+                  final IH. Since we got here from withdrawal we will be in left case. *)
+              rewrite seller_done in *.
+              left.
+              repeat rewrite transfer_acts_to_cons.
+              fold (buyer_confirmed prev_inc_calls
+                                    (setup_buyer (deployment_setup dep_info))).
+              destruct IH as [_ [_ [<- [-> [? [_ [-> [[? ->] [? ?]]]]]]]]].
+              rewrite address_eq_refl.
+              rewrite address_eq_ne by assumption.
+              cbn.
+              do 2 (split; [eauto|]).
+              lia.
+            ++ (* Seller still has more to withdraw, next_step is still withdrawals *)
+              cbn.
+              rewrite prev_next_step.
+              repeat rewrite transfer_acts_to_cons.
+              fold (buyer_confirmed prev_inc_calls
+                                    (setup_buyer (deployment_setup dep_info))).
+              destruct IH as [_ [_ [<- [-> [? [_ [-> [[? ->] [? ?]]]]]]]]].
+              rewrite address_eq_refl.
+              rewrite address_eq_ne by assumption.
+              cbn.
+              do 2 (split; eauto).
+              lia.
+          -- (* Seller withdrawing. Todo: generalize and clean up. *)
+            cbn in *.
+            destruct_match in receive_some; cbn in *; try congruence.
+            inversion_clear receive_some; cbn.
+            apply and_assoc; split; [destruct_match; tauto|].
+            do 2 (split; try tauto).
+            destruct (Z.eqb_spec (buyer_withdrawable prev_state) 0) as [buyer_done|].
+            ++ (* No one has more to withdrew, next_step is no_next_step now, so establish
+                  final IH. Since we got here from withdrawal we will be in left case. *)
+              rewrite buyer_done in *.
+              left.
+              repeat rewrite transfer_acts_to_cons.
+              fold (buyer_confirmed prev_inc_calls
+                                    (setup_buyer (deployment_setup dep_info))).
+              destruct IH as [_ [_ [<- [<- [? [_ [-> [[? ->] [? ?]]]]]]]]].
+              rewrite address_eq_refl.
+              rewrite address_eq_ne by auto.
+              cbn.
+              do 2 (split; eauto).
+              lia.
+            ++ (* Buyer still has more to withdraw, next_step is still withdrawals *)
+              cbn.
+              rewrite prev_next_step.
+              repeat rewrite transfer_acts_to_cons.
+              fold (buyer_confirmed prev_inc_calls
+                                    (setup_buyer (deployment_setup dep_info))).
+              destruct IH as [_ [_ [<- [<- [? [_ [-> [[? ->] [? ?]]]]]]]]].
+              rewrite address_eq_refl.
+              rewrite address_eq_ne by auto.
+              cbn.
+              do 2 (split; eauto).
+              lia.
+      + (* None *)
+        congruence.
+    - (* Self call *)
+      instantiate (CallFacts := fun _ ctx _ _ => ctx_from ctx <> ctx_contract_address ctx);
+        subst CallFacts; cbn in *; congruence.
+    - (* Permuting queue *)
+      do 5 (split; try tauto).
+      split.
+      + now rewrite <- perm.
+      + assert (out_queue = [] -> out_queue' = [])
+          by (intros ->; now apply Permutation_nil).
+        unfold transfer_acts_to in *.
+        repeat rewrite sumZ_filter in *.
+        destruct (next_step cstate); try tauto.
+        * now rewrite <- perm.
+        * destruct IH as [_ [_ [_ [_ [_ [_ [IH | IH]]]]]]];
+            [left|right]; rewrite <- perm; auto.
+    - instantiate (AddBlockFacts := fun _ _ _ _ _ _ => True).
+      unset_all; subst; cbn in *.
+      destruct_chain_step; auto.
+      destruct_action_eval; auto.
+      intros.
+      pose proof (no_self_calls bstate_from to_addr ltac:(assumption) ltac:(assumption))
+           as all.
+      unfold outgoing_acts in *.
+      rewrite queue_prev in *.
+      subst act; cbn in all.
+      destruct_address_eq; cbn in *; auto.
+      inversion_clear all as [|? ? hd _].
+      destruct msg.
+      + contradiction.
+      + rewrite address_eq_refl in hd.
+        congruence.
+  Qed.
+
+  Definition net_balance_effect
+             {bstate_from bstate_to : ChainState}
+             (trace : ChainTrace bstate_from bstate_to)
+             (caddr addr : Address) : Amount :=
+    sumZ tx_amount (txs_to addr (outgoing_txs trace caddr))
+    - sumZ tx_amount (txs_from addr (incoming_txs trace caddr)).
+
+  (* Our main assumption is that the escrow will always finish due to
+  economically rational actors. We do not formalize this. *)
+  Definition is_escrow_finished cstate :=
+    match next_step cstate with
+    | no_next_step => true
+    | _ => false
+    end.
+
+  (* The functional correctness of the Escrow, under the assumption that the
+  escrow finishes due to rational actors. *)
+  Corollary escrow_correct
+            {ChainBuilder : ChainBuilderType}
+            prev new header acts :
+    builder_add_block prev header acts = Ok new ->
+    let trace := builder_trace new in
+    forall caddr,
+      env_contracts new caddr = Some (Escrow.contract : WeakContract) ->
+      exists (depinfo : DeploymentInfo Setup)
+             (cstate : State)
+             (inc_calls : list (ContractCallInfo Msg)),
+        deployment_info Setup trace caddr = Some depinfo /\
+        contract_state new caddr = Some cstate /\
+        incoming_calls Msg trace caddr = Some inc_calls /\
+        let item_worth := deployment_amount depinfo / 2 in
+        let seller := deployment_from depinfo in
+        let buyer := setup_buyer (deployment_setup depinfo) in
+        is_escrow_finished cstate = true ->
+        (buyer_confirmed inc_calls buyer = true /\
+         net_balance_effect trace caddr seller = item_worth /\
+         net_balance_effect trace caddr buyer = -item_worth \/
+
+         buyer_confirmed inc_calls buyer = false /\
+         net_balance_effect trace caddr seller = 0 /\
+         net_balance_effect trace caddr buyer = 0).
+  Proof.
+    intros after_add trace caddr escrow_at_caddr.
+    cbn in *.
+    pose proof (escrow_correct_strong _ caddr trace escrow_at_caddr) as general.
+    cbn in general.
+    destruct general as
+        [cstate [depinfo [inc_calls [? [? [? [? [? [? [? [? [_ IH]]]]]]]]]]]].
+    exists depinfo, cstate, inc_calls.
+    do 3 (split; [tauto|]).
+    intros is_finished.
+    unfold is_escrow_finished in *.
+    destruct (next_step cstate); try congruence; clear is_finished.
+    unfold net_balance_effect, money_to.
+    assert (inc_txs:
+              forall addr,
+                sumZ tx_amount (txs_from addr (incoming_txs trace caddr)) =
+                sumZ (fun '(a, b, c) => c)
+                     (filter (fun '(from, _, _) => (from =? addr)%address)
+                             (map (fun tx => (tx_from tx, tx_to tx, tx_amount tx))
+                                  (incoming_txs trace caddr)))).
+    {
+      intros addr.
+      induction (incoming_txs trace caddr) as [|hd tl IH'].
+      - reflexivity.
+      - rewrite txs_from_cons.
+        cbn.
+        destruct_address_eq; cbn in *; rewrite IH'; reflexivity.
+    }
+
+    repeat rewrite inc_txs; clear inc_txs.
+    rewrite (incoming_txs_contract caddr _ trace _ depinfo _ inc_calls) by assumption.
+    repeat rewrite filter_app, sumZ_app.
+    cbn.
+    rewrite address_eq_refl.
+    rewrite address_eq_ne by auto.
+    cbn.
+    rewrite 2!filter_map, 2!sumZ_map.
+
+    set (buyer_addr := setup_buyer (deployment_setup depinfo)) in *.
+    set (seller_addr := deployment_from depinfo) in *.
+
+    unfold money_to, transfer_acts_to in IH.
+    cbn in IH.
+
+    change (fun a => call_amount a) with (@call_amount _ Msg).
+
+    destruct IH as [IH | IH]; [left|right].
+    - split; [tauto|].
+      destruct IH as [_ [[origin HH] ?]].
+      remember (build_call_info _ _ _ (Some commit_money)) as commitment.
+      assert (Hsum :
+                forall f,
+                  sumZ call_amount (filter f inc_calls) =
+                  sumZ call_amount (filter f [commitment])).
+      {
+        intros f.
+        rewrite <- HH.
+        clear -inc_calls.
+        induction inc_calls as [|hd tl IH']; auto.
+        cbn.
+        destruct (Z.eqb_spec (call_amount hd) 0) as [zero_amount|].
+        - cbn.
+          destruct (f hd); cbn; try rewrite zero_amount; rewrite IH'; auto.
+        - cbn.
+          destruct (f hd); cbn; rewrite IH'; auto.
+      }
+
+      rewrite 2!Hsum; clear Hsum; subst commitment; cbn in *.
+      rewrite address_eq_refl, address_eq_ne by auto.
+      cbn.
+      split; lia.
+    - destruct IH as [[? ->] IH].
+      cbn.
+      rewrite address_eq_refl, address_eq_ne by auto.
+      cbn.
+      split; [auto|].
+      split; lia.
+  Qed.
+
+End Theories.
+
+End EscrowSolana.
