extraction/theories/SolanaExtract.v
@@ -1,0 +1,501 @@
+From MetaCoq Require Import utils.
+From MetaCoq.Template Require Import All.
+From MetaCoq.Template Require Import Kernames.
+From ConCert.Utils Require Import StringExtra.
+From ConCert.Execution Require Import BlockchainSolana.
+From ConCert.Extraction Require Import Common.
+From ConCert.Extraction Require Import Extraction.
+From ConCert.Extraction Require Import RustExtract.
+From ConCert.Extraction Require Import Optimize.
+From ConCert.Extraction Require Import SpecializeChainBaseSolana.
+From ConCert.Extraction Require Import PrettyPrinterMonad.
+From ConCert.Extraction Require Import Printing.
+From ConCert.Extraction Require Import ResultMonad.
+From ConCert.Extraction Require Import Utils.
+
+Module SolanaRemap.
+
+Definition lookup_const (TT : list (kername * string)) (name : kername): option string :=
+  match find (fun '(key, _) => eq_kername key name) TT with
+  | Some (_, val) => Some val
+  | None => None
+  end.
+
+Definition remap_arith : list (kername * string) := Eval compute in
+  [  remap <%% BinPosDef.Pos.add %%> "fn ##name##(&'a self, a: u64, b: u64) -> u64 { a.checked_add(b).unwrap() }"
+   ; remap <%% BinPosDef.Pos.succ %%> "fn ##name##(&'a self, a: u64) -> u64 { a.checked_add(1).unwrap() }"
+   ; remap <%% Z.add %%> "fn ##name##(&'a self, a: i64, b: i64) -> i64 { a.checked_add(b).unwrap() }"
+   ; remap <%% Z.sub %%> "fn ##name##(&'a self, a: i64, b: i64) -> i64 { a.checked_sub(b).unwrap() }"
+   ; remap <%% Z.mul %%> "fn ##name##(&'a self, a: i64, b: i64) -> i64 { a.checked_mul(b).unwrap() }"
+   ; remap <%% BinIntDef.Z.even %%> "fn ##name##(&'a self, a: i64) -> bool { a.checked_rem(2).unwrap() == 0 }"
+   ; remap <%% BinIntDef.Z.odd %%> "fn ##name##(&'a self, a: i64) -> bool { a.checked_rem(2).unwrap() != 0 }"
+   ; remap <%% Z.eqb %%> "fn ##name##(&'a self, a: i64, b: i64) -> bool { a == b }"
+   ; remap <%% Z.leb %%> "fn ##name##(&'a self, a: i64, b: i64) -> bool { a <= b }"
+   ; remap <%% Z.ltb %%> "fn ##name##(&'a self, a: i64, b: i64) -> bool { a < b }"
+   ; remap <%% Z.gtb %%> "fn ##name##(&'a self, a: i64, b: i64) -> bool { a > b }"
+   ; remap <%% Nat.add %%> "fn ##name##(&'a self, a: u64, b: u64) -> u64 { a.checked_add(b).unwrap() }"
+   ; remap <%% Nat.leb %%> "fn ##name##(&'a self, a: u64, b: u64) -> bool { a <= b }"
+   ; remap <%% Nat.ltb %%> "fn ##name##(&'a self, a: u64, b: u64) -> bool { a < b }"].
+
+(* J> DONE: Changed the address and address_eq from concordium_std to solana_program *)
+Definition remap_blockchain_consts : list (kername * string) :=
+  [ remap <! @Address !> "type ##name##<'a> = solana_program::pubkey::Pubkey;"
+  (* Ideally we would have two impls here for performance, but Rust does not support this.
+     https://github.com/rust-lang/rust/issues/62223 *)
+  ; remap <! @address_eqb !>
+          "fn ##name##(&'a self) -> impl Fn(solana_program::pubkey::Pubkey) -> &'a dyn Fn(solana_program::pubkey::Pubkey) -> bool { move |a| self.alloc(move |b| a == b) }" ].
+
+Definition remap_inline_bool_ops := Eval compute in
+      [ remap <%% andb %%> "__andb!"
+      ; remap <%% orb %%> "__orb!"].
+
+Definition remap_nat : remapped_inductive:=
+  {| re_ind_name := "u64";
+     re_ind_ctors := ["0"; "__nat_succ"];
+     re_ind_match := Some "__nat_elim!" |}.
+
+Definition remap_positive : remapped_inductive :=
+  {| re_ind_name := "u64";
+     re_ind_ctors := ["__pos_onebit"; "__pos_zerobit"; "1"];
+     re_ind_match := Some "__pos_elim!"
+  |}.
+
+Definition remap_Z : remapped_inductive :=
+  {| re_ind_name := "i64";
+     re_ind_ctors := ["0"; "__Z_frompos"; "__Z_fromneg"];
+     re_ind_match := Some "__Z_elim!";
+  |}.
+
+Definition remap_bool : remapped_inductive :=
+  {| re_ind_name := "bool";
+     re_ind_ctors := ["true"; "false"];
+     re_ind_match := None
+  |}.
+
+Definition remap_pair : remapped_inductive :=
+  {| re_ind_name := "__pair";
+     re_ind_ctors := ["__mk_pair"];
+     re_ind_match := Some "__pair_elim!"
+  |}.
+
+Definition remap_option : remapped_inductive :=
+  {| re_ind_name := "Option";
+     re_ind_ctors := ["Some"; "None"];
+     re_ind_match := None
+  |}.
+
+Definition remap_unit : remapped_inductive :=
+  {| re_ind_name := "()";
+     re_ind_ctors := ["()"];
+     re_ind_match := None
+  |}.
+
+Definition remap_string : remapped_inductive :=
+  {| re_ind_name := "&'a String";
+     re_ind_ctors := [];
+     re_ind_match := None |}.
+
+Definition remap_std_types :=
+  [ (<! nat !>, remap_nat)
+  ; (<! positive !>, remap_positive)
+  ; (<! Z !>,  remap_Z)
+  ; (<! bool !>, remap_bool)
+  ; (<! prod !>, remap_pair)
+  ; (<! option !>, remap_option)
+  ; (<! unit !>, remap_unit)
+  ; (<! string !>, remap_string) ].
+
+Definition remap_SerializedValue : remapped_inductive :=
+  {| re_ind_name := "&'a SerializedValue<'a>";
+     re_ind_ctors := ["__SerializedValue__Is__Opaque"];
+     re_ind_match := None |}.
+
+Definition remap_ActionBody : remapped_inductive :=
+  {| re_ind_name := "ActionBody<'a>";
+     re_ind_ctors := ["ActionBody::Transfer"; "ActionBody::Call"; "__Deploy__Is__Not__Supported"; "ActionBody::SpecialCall"];
+     re_ind_match := None |}.
+
+Definition remap_SpecialCallBody : remapped_inductive := 
+  {| re_ind_name := "SpecialCallBody<'a>";
+     re_ind_ctors := ["SpecialCallBody::TransferOwnership"];  
+     re_ind_match := None |}.
+
+Definition remap_blockchain_inductives : list (inductive * remapped_inductive) :=
+  [ (<! Serializable.SerializedValue !>, remap_SerializedValue);
+    (<! @ActionBody !>, remap_ActionBody);
+    (<! @SpecialCallBody !>, remap_SpecialCallBody) ].
+
+Definition ignored_concert :=
+  [ <%% Monads.Monad %%>; <%% @RecordSet.SetterFromGetter %%> ].
+
+Definition lookup_inductive
+           (TT_inductives : list (inductive * remapped_inductive))
+           (ind : inductive) : option remapped_inductive :=
+  match find (fun '(key, _) => eq_inductive key ind) TT_inductives with
+  | Some (_, val) => Some val
+  | None => None
+  end.
+
+Definition build_remaps
+           (TT_const : list (kername * string))
+           (TT_const_inline : list (kername * string))
+           (TT_inductives : list (inductive * remapped_inductive))
+  : remaps :=
+  {| remap_inductive := lookup_inductive TT_inductives;
+     remap_constant := lookup_const TT_const;
+     remap_inline_constant := lookup_const TT_const_inline; |}.
+
+End SolanaRemap.
+
+Module SolanaPreamble.
+Instance solana_extract_preamble : Preamble :=
+(* J> TODO: Update: probably just need to update the errors near the end *)
+{| top_preamble := [
+"#![allow(dead_code)]";
+"#![allow(non_camel_case_types)]";
+"#![allow(unused_imports)]";
+"#![allow(non_snake_case)]";
+"#![allow(unused_variables)]";
+"";
+"use solana_program::{";
+"  account_info::{next_account_info, AccountInfo},";
+"  clock::Clock,";
+"  entrypoint,";
+"  entrypoint::ProgramResult,";
+"  msg,";
+"  program_error::ProgramError,";
+"  pubkey::Pubkey,";
+"  rent::Rent,";
+"  sysvar::Sysvar,";
+"};";
+"use ::borsh::{BorshSerialize, BorshDeserialize};";
+"use concert_std::{ActionBody, ConCertDeserial, ConCertSerial, SerializedValue};";
+"use core::marker::PhantomData;";
+"use immutable_map::TreeMap;"; 
+"use spl_token::state::Account as TokenAccount;";
+"";
+"fn __nat_succ(x: u64) -> u64 {";
+"  x.checked_add(1).unwrap()";
+"}";
+"";
+"macro_rules! __nat_elim {";
+"    ($zcase:expr, $pred:ident, $scase:expr, $val:expr) => {";
+"        { let v = $val;";
+"        if v == 0 { $zcase } else { let $pred = v - 1; $scase } }";
+"    }";
+"}";
+"";
+"macro_rules! __andb { ($b1:expr, $b2:expr) => { $b1 && $b2 } }";
+"macro_rules! __orb { ($b1:expr, $b2:expr) => { $b1 || $b2 } }";
+"";
+"fn __pos_onebit(x: u64) -> u64 {";
+"  x.checked_mul(2).unwrap() + 1";
+"}";
+"";
+"fn __pos_zerobit(x: u64) -> u64 {";
+"  x.checked_mul(2).unwrap()";
+"}";
+"";
+"macro_rules! __pos_elim {";
+"    ($p:ident, $onebcase:expr, $p2:ident, $zerobcase:expr, $onecase:expr, $val:expr) => {";
+"        {";
+"            let n = $val;";
+"            if n == 1 {";
+"                $onecase";
+"            } else if (n & 1) == 0 {";
+"                let $p2 = n >> 1;";
+"                $zerobcase";
+"            } else {";
+"                let $p = n >> 1;";
+"                $onebcase";
+"            }";
+"        }";
+"    }";
+"}";
+"";
+"fn __Z_frompos(z: u64) -> i64 {";
+"  use std::convert::TryFrom;";
+"";
+"  i64::try_from(z).unwrap()";
+"}";
+"";
+"fn __Z_fromneg(z : u64) -> i64 {";
+"  use std::convert::TryFrom;";
+"";
+"  i64::try_from(z).unwrap().checked_neg().unwrap()";
+"}";
+"";
+"macro_rules! __Z_elim {";
+"    ($zero_case:expr, $p:ident, $pos_case:expr, $p2:ident, $neg_case:expr, $val:expr) => {";
+"        {";
+"            let n = $val;";
+"            if n == 0 {";
+"                $zero_case";
+"            } else if n < 0 {";
+"                let $p2 = n.unsigned_abs();";
+"                $neg_case";
+"            } else {";
+"                let $p = n as u64;";
+"                $pos_case";
+"            }";
+"        }";
+"    }";
+"}";
+"";
+"fn __N_frompos(z: u64) -> u64 {";
+"  z";
+"}";
+"";
+"macro_rules! __N_elim {";
+"    ($zero_case:expr, $p:ident, $pos_case:expr, $val:expr) => {";
+"        { let $p = $val; if $p == 0 { $zero_case } else { $pos_case } }";
+"    }";
+"}";
+"";
+"type __pair<A, B> = (A, B);";
+"";
+"macro_rules! __pair_elim {";
+"    ($fst:ident, $snd:ident, $body:expr, $p:expr) => {";
+"        { let ($fst, $snd) = $p; $body }";
+"    }";
+"}";
+"";
+"fn __mk_pair<A: Copy, B: Copy>(a: A, b: B) -> __pair<A, B> { (a, b) }";
+"";
+"fn hint_app<TArg, TRet>(f: &dyn Fn(TArg) -> TRet) -> &dyn Fn(TArg) -> TRet {";
+"  f";
+"}";
+"";
+"#[derive(Debug, PartialEq, Eq)]";
+"enum InitError {";
+"   DeserialParams,";
+"   SerialParams,";
+"   Error";
+"}";
+"";
+"#[derive(Debug, PartialEq, Eq)]";
+"enum ReceiveError {";
+"    DeserialMsg,";
+"    DeserialOldState,";
+"    SerialNewState,";
+"    ConvertActions, // Cannot convert ConCert actions to Concordium actions";
+"    Error";
+"}"
+];
+program_preamble := [
+"fn alloc<T>(&'a self, t: T) -> &'a T {";
+"  self.__alloc.alloc(t)";
+"}";
+"";
+"fn closure<TArg, TRet>(&'a self, F: impl Fn(TArg) -> TRet + 'a) -> &'a dyn Fn(TArg) -> TRet {";
+"  self.__alloc.alloc(F)";
+"}" ] |}.
+
+End SolanaPreamble.
+
+Import SolanaRemap.
+
+(* J> TODO: Modify types *)
+Record SolanaMod (init_type receive_type : Type) :=
+  { solana_contract_name : string;
+    solana_init : init_type;
+    solana_receive : receive_type;
+    solana_extra : list ({T : Type & T}); }.
+
+Arguments solana_contract_name {_ _}.
+Arguments solana_init {_ _}.
+Arguments solana_receive {_ _}.
+Arguments solana_extra {_ _}.
+
+Definition get_fn_arg_type (Σ : Ex.global_env) (fn_name : kername) (n : nat)
+  : result Ex.box_type string :=
+  match Ex.lookup_env Σ fn_name with
+  | Some (Ex.ConstantDecl cb) =>
+    match decompose_TArr cb.(Ex.cst_type).2 with
+    | (tys, _) => result_of_option (nth_error tys n)
+                                  ("No argument at position " ++ string_of_nat n)
+    end
+  | _ => Err "Init declaration must be a constant in the global environment"
+  end.
+
+Definition specialize_extract_template_env
+           (params : extract_template_env_params)
+           (Σ : global_env)
+           (seeds : KernameSet.t)
+           (ignore : kername -> bool) : result ExAst.global_env string :=
+  extract_template_env_general SpecializeChainBaseSolana.specialize_ChainBase_env
+                       params
+                       Σ
+                       seeds
+                       ignore.
+
+Section SolanaPrinting.
+
+  Context `{RustPrintConfig}.
+
+  Definition extract_lines
+             (seeds : KernameSet.t)
+             (Σ : global_env)
+             (remaps : remaps)
+             (params : extract_template_env_params) : result (list string) string :=
+    let should_ignore kn :=
+        if remap_inductive remaps (mkInd kn 0) then true else
+        if remap_constant remaps kn then true else
+        if remap_inline_constant remaps kn then true else false in
+    Σ <- specialize_extract_template_env params Σ seeds should_ignore;;
+    let attrs _ := "#[derive(Clone, ConCertSerial, ConCertDeserial, PartialEq)]" in
+    let p := print_program Σ remaps attrs in
+    '(_, s) <- timed "Printing" (fun _ => finish_print_lines p);;
+    ret s.
+
+  Open Scope string.
+
+  (* TODO: Modify all of this *)
+
+  Definition process_instruction_wrapper (receive_name : kername) := 
+(* J> Instruction info should have NAMES and PARAMETERS *)
+(* J> This chain definition seems to be good and according to the execution model *)
+    <$
+      "fn process_instruction (";
+      "    program_id: &Pubkey,";
+      "    accounts: &[AccountInfo],";
+      "    instruction_data: &[u8],";
+      ") -> ProgramResult {";
+      "    let prg = Program::new();";
+      "    let msg =";
+      "        match <_>::concert_deserial(&mut ctx.parameter_cursor(), &prg.__alloc) {";
+      "            Ok(m) => m,";
+      "            Err(_) => return Err(ReceiveError::DeserialMsg)";
+      "        };";
+      "    let old_state =";
+      "        match <_>::concert_deserial(state, &prg.__alloc) {";
+      "            Ok(s) => s,";
+      "            Err(_) => return Err(ReceiveError::DeserialOldState)";
+      "        };";
+      "    let cchain ="; 
+      "        " ++ RustExtract.ty_const_global_ident_of_kername <%% Chain %%> ++ "::build_chain(";
+      "            PhantomData,";
+      "            0, // No chain height";
+      "            Clock::get().unix_timestamp,";
+      "            0 // No finalized height";
+      "        );";
+      "    let balance = if ctx.sender() != concordium_std::Address::Contract(ctx.self_address()) {";
+      "   // if the contract is not calling itself, we add amount to the current balance";
+      "   // as expeced by the ConCert execution model";
+      "   (ctx.self_balance().micro_ccd + amount.micro_ccd) as i64";
+      "    } else {";
+      "        ctx.self_balance().micro_ccd as i64";
+      "    };";
+      "    let cctx =";
+      "        " ++ RustExtract.ty_const_global_ident_of_kername <%% @ContractCallContext %%> ++ "::build_ctx(" $>.
+      "            PhantomData,";
+      "            Address::Account(ctx.invoker()),";
+      "            ctx.sender(),";
+      "            Address::Contract(ctx.self_address()),";
+      "            balance,";
+      "            amount.micro_ccd as i64);";
+      "    let res = prg." ++ RustExtract.const_global_ident_of_kername receive_name ++ "(&cchain, &cctx, old_state, msg);";
+      "    match res {";
+      "        Option::Some((new_state, acts)) => {";
+      "            state.truncate(0);";
+      "            match new_state.concert_serial(state) {";
+      "                Ok(_) => convert_actions(acts),";
+      "                Err(_) => Err(ReceiveError::SerialNewState)";
+      "            }";
+      "        }";
+      "        Option::None => Err(ReceiveError::Error)";
+      "    }";
+      "}" ;
+      "entrypoint!(process_instruction);" $>.
+
+  Definition list_name : string :=
+    RustExtract.ty_const_global_ident_of_kername <%% list %%>.
+
+(*J> TODO: adjust returns and return type *)
+
+  Definition convert_special_action : string :=
+  <$
+"fn convert_special_action(body: &SpecialCallBody) -> Result<(), ReceiveError> {";
+"  match body { ";
+"                     ";
+"                     ";
+"                     ";
+"                     ";
+"                     ";
+"                     ";
+"                     ";
+"                     ";
+"  }";
+"}" $>.
+
+  Definition convert_actions : string :=
+  <$
+"fn convert_actions(acts: &" ++ list_name ++ "<ActionBody>) -> Result<(), ReceiveError> {";
+"  match acts {";
+"    &" ++ list_name ++ "::nil(_) => Ok(()),";
+"    &" ++ list_name ++ "::cons(_, hd, tl) => {";
+"    let cact =";
+"        if let ActionBody::Transfer(donator_account, receiver_account, amount) = hd {";
+"            if **donator_account.try_borrow_mut_lamports()? >= amount {";
+"               **receiver_account.try_borrow_mut_lamports()? += amount;";
+"               **donator_account.try_borrow_mut_lamports()? -= amount;";
+"            } else {";
+"               return Err(ReceiveError::Error)";
+"            };"; 
+"        if let ActionBody::SpecialCall(to, body) = hd {";
+"            convert_special_action(body);";
+"        } else {";
+"            return Err(ReceiveError::ConvertActions)";
+"        };";
+"      Ok(())";
+"    }";
+"  }";
+"}" $>.
+
+(*   Definition print_receive_attrs (contract_name : string) (receive_name : kername) : string :=
+    "#[receive(contract = """ ++ contract_name ++ """" ++
+              ", name = """ ++ RustExtract.const_global_ident_of_kername receive_name ++ """" ++
+              ", payable, enable_logger, low_level)]". *)
+
+Definition print_lines (lines : list string) : TemplateMonad unit :=
+    monad_iter tmMsg lines.
+
+(* TODO : Update this definition *)
+Definition solana_extraction
+           {init_type receive_type : Type}
+           (m : SolanaMod init_type receive_type)
+           (remaps : remaps)
+           (should_inline : kername -> bool) : TemplateMonad _ :=
+  init_tm <- tmEval cbn m.(solana_init);;
+  recv_tm <- tmEval cbn m.(solana_receive);;
+  '(Σ,_) <- tmQuoteRecTransp (init_tm, recv_tm) false ;;
+  init_nm <- extract_def_name m.(solana_init);;
+  receive_nm <- extract_def_name m.(solana_receive);;
+  extra <- monad_map extract_def_name_exists m.(solana_extra);;
+  let overridden_masks kn :=
+      if eq_kername kn init_nm || eq_kername kn receive_nm then
+        Some []
+      else
+        None in
+  let seeds := KernameSetProp.of_list (init_nm :: receive_nm :: extra) in
+  let params := extract_rust_within_coq overridden_masks should_inline in
+  Σ <- run_transforms Σ params;;
+  res <- tmEval lazy (extract_lines seeds Σ remaps params);;
+  match res with
+  | Ok lines =>
+    let process_wrapper := process_instruction_wrapper init_nm in
+    print_lines (lines ++ [""; convert_actions; ""; process_wrapper])
+  | Err e => tmFail e
+  end.
+
+End SolanaPrinting.
+
+Module DefaultPrintConfig.
+
+  Definition RustConfig : RustPrintConfig :=
+    {| term_box_symbol := "()";
+       type_box_symbol := "()";
+       any_type_symbol := "()";
+       print_full_names := true |}.
+
+End DefaultPrintConfig.
